src/Parsers/NonComputational.v
@@ -135,10 +135,6 @@ Local Open Scope string_like_scope.
 
 Section recursive_descent_parser.
   Context CharType (String : string_like CharType) (G : grammar CharType).
-  (** FIXME: The type of the list of nonterminals should be able to
-  depend on the string we're parsing, so we can store proofs in it to
-  pass down the parse tree to handle impossible cases.  This will
-  require a [Total] lexicographic ordering on strings. *)
   Context (nonterminal_listT : String -> Type)
           (initial_nonterminal_data : forall str, nonterminal_listT str)
           (is_valid_nonterminal : forall str, nonterminal_listT str -> nonterminal CharType -> bool)
@@ -148,8 +144,22 @@ Section recursive_descent_parser.
                                                   -> nonterminal_listT_R str (remove_nonterminal str ls nt) ls)
           (ntl_wf : forall str, well_founded (nonterminal_listT_R str)).
   Section generic.
-    Context (T : String -> nonterminal CharType -> Type)
-            (T_reverse_lookup : forall str name, T str (Lookup G name) -> T str [ [ NonTerminal _ name ] ]).
+    Context (T_success T_failure : String -> nonterminal CharType -> Type)
+            (T_success_reverse_lookup : forall str name, T_success str (Lookup G name) -> T_success str [ [ NonTerminal _ name ] ])
+            (T_failure_reverse_lookup : forall str name, T_failure str (Lookup G name) -> T_failure str [ [ NonTerminal _ name ] ])
+            (transport_T_success_str : forall (s1 s2 : String) nt, s1 = s2 -> T_success s1 nt -> T_success s2 nt)
+            (transport_T_failure_str : forall (s1 s2 : String) nt, s1 = s2 -> T_failure s1 nt -> T_failure s2 nt).
+    Let T str nt := (T_success str nt + T_failure str nt)%type.
+    Let transport_T_str (s1 s2 : String) nt (H : s1 = s2) (p : T s1 nt) : T s2 nt :=
+      match p with
+        | inl p' => inl (transport_T_success_str H p')
+        | inr p' => inr (transport_T_failure_str H p')
+      end.
+    Let T_reverse_lookup str name (p : T str (Lookup G name)) : T str [ [ NonTerminal _ name ] ]
+      :=  match p with
+            | inl p' => inl (T_success_reverse_lookup _ p')
+            | inr p' => inr (T_failure_reverse_lookup _ p')
+          end.
     Context (parse_pattern_by_picking
              : forall str0
                       (parse_pattern_from_split_list'
@@ -164,7 +174,7 @@ Section recursive_descent_parser.
     Context (fold_patterns : forall str (pats : list (pattern CharType)),
                                ilist (fun pat => T str [ pat ]) pats
                                -> T str pats).
-    Context (make_abort : forall str nt valid_list, @is_valid_nonterminal str valid_list nt = false -> T str nt).
+    Context (make_abort : forall str nt valid_list, @is_valid_nonterminal str valid_list nt = false -> T_failure str nt).
 
 
     Section parts.
@@ -231,7 +241,7 @@ Section recursive_descent_parser.
                          _ _).
             intros [str0 valid_list] parse_nonterminal str pf nt; simpl in *.
             destruct (lt_dec (Length _ str) (Length _ str0)) as [pf'|pf'];
-              [ | assert (str = str0) by intuition; subst ].
+              [ | assert (H : str0 = str) by intuition; apply (transport_T_str H); clear H ].
             { (** [str] got smaller, so we reset the valid nonterminals *)
               specialize (parse_nonterminal
                             (existT _ str (initial_nonterminal_data str))
@@ -240,14 +250,14 @@ Section recursive_descent_parser.
             { (** [str] didn't get smaller, so we cache the fact that we've hit this nonterminal already *)
               case_eq (is_valid_nonterminal valid_list nt).
               { (** It was valid, so we can remove it *)
-                intro H.
+                intro H'.
                 specialize (fun pf' => parse_nonterminal
                               (existT _ str0 (remove_nonterminal valid_list nt))
                               (or_intror (ex_intro _ eq_refl pf'))); simpl in *.
-                specialize (parse_nonterminal (remove_nonterminal_dec H)).
+                specialize (parse_nonterminal (remove_nonterminal_dec H')).
                 exact (parse_nonterminal_step parse_nonterminal (or_intror eq_refl) nt). }
               { (** oops, we already saw this nonterminal in the past.  ABORT! *)
-                apply make_abort. } }
+                intro; right; eapply make_abort; eassumption. } }
           Defined.
 
           Definition parse_nonterminal str nt : T str nt
@@ -257,6 +267,304 @@ Section recursive_descent_parser.
       End nonterminal.
     End parts.
   End generic.
+
+  Section parse_tree.
+    Local Hint Constructors parse_of parse_of_pattern parse_of_item : parse_tree.
+    Local Hint Resolve ParseHead ParsePatternSingleton : parse_tree.
+    Local Hint Extern 1 => apply ParseHead : parse_tree.
+    Local Hint Extern 0 (option (parse_of _ _ _ [])) => exact None : parse_tree.
+    Context (pick_patterns
+             : forall (str : String)
+                      (pat : pattern CharType)
+                      (patH : Datatypes.length pat > 0),
+                 { ls : list { split : list { str_part : String | Length _ str_part < Length _ str \/ str_part = str }
+                             | List.length split = List.length pat
+                               /\ fold_right (Concat _) (Empty _) (map (@proj1_sig _ _) split) = str }
+                 | List.length ls <> 0 }).
+
+    Let aggregate str pats : list (parse_of String G str pats +
+                                   option (parse_of String G str pats -> False))
+                             -> parse_of String G str pats +
+                                option (parse_of String G str pats -> False).
+    Proof.
+      intro ls.
+      induction ls as [|x xs IHxs].
+      { right; exact None. }
+      { destruct x as [| [ ] ]; try solve [ left; assumption
+                                          | right; apply Some; assumption ].
+        apply IHxs. }
+    Defined.
+
+    Definition parse_tree_for : forall str nt, parse_of String G str nt + option (parse_of String G str nt -> False).
+    Proof with auto with parse_tree nocore.
+      apply (@parse_nonterminal (fun str nt => parse_of _ G str nt)
+                                (fun str nt => option (parse_of _ G str nt -> False)))...
+      { intros str name [np|]; [ apply Some | exact None ].
+        revert np; clear; intros.
+        abstract (repeat match goal with
+                           | [ H : context[_ ++ Empty String] |- _ ] => rewrite RightId in H
+                           | [ H : ?T, H' : ?T -> False |- _ ] => destruct (H' H)
+                           | [ p : parse_of _ _ _ _ |- _ ] => (inversion p; subst; clear p)
+                           | [ p : parse_of_pattern _ _ _ _ |- _ ] => (inversion p; subst; clear p)
+                           | [ p : parse_of_item _ _ _ _ |- _ ] => (inversion p; subst; clear p)
+                         end). }
+        { intros; subst; assumption. }
+        { intros; subst; assumption. }
+        { intros str0 parse_pattern_from_split_list' str pf pat.
+          pose proof (parse_pattern_from_split_list' ((exist _ str pf)::nil) pat) as parse_pattern_from_split_list''; simpl in *.
+          destruct pat as [|pat0 [|pat1 pats] ]; simpl in *.
+          { case_eq (str =s Empty _); intro H; [ left | right; exact None ]...
+            apply bool_eq_correct in H; subst... }
+          { destruct (ilist_hd parse_pattern_from_split_list'') as [tree|]; simpl in *; [ left | right ]; assumption. }
+          { (** we need to split the string *)
+            clear parse_pattern_from_split_list''.
+            refine (aggregate _); clear aggregate.
+            refine (map _ (proj1_sig (@pick_patterns str (pat0::pat1::pats) (Gt.gt_Sn_O _)))); clear pick_patterns.
+            intros [ split [ split_length split_strings ] ].
+            let T := match type of split with list ?T => constr:(T) end in
+            set (f := (map (fun x' : T
+                      => exist
+                           (fun str => Length String str < Length String str0 \/ str = str0)
+                           (proj1_sig x')
+                           (match pf, proj2_sig x' with
+                              | or_introl H0, or_introl H1 => or_introl (transitivity H1 H0)
+                              | or_introl H0, or_intror H1 => or_introl (transitivity (R := le) (Le.le_n_S _ _ (NPeano.Nat.eq_le_incl _ _ (f_equal (Length String) H1))) H0)
+                              | or_intror H0, or_introl H1 => or_introl (transitivity (R := le) H1 (NPeano.Nat.eq_le_incl _ _ (f_equal (Length String) H0)))
+                              | or_intror H0, or_intror H1 => or_intror (transitivity H1 H0)
+                            end)))).
+            specialize (parse_pattern_from_split_list' (f split) (pat0 :: pat1 :: pats)).
+            generalize dependent split.
+            intro split.
+            generalize (pat0::pat1::pats).
+            clear pat0 pat1 pats.
+            assert (H0 : Datatypes.length (f split) = Datatypes.length split)
+              by (clear; abstract (induction split; simpl; auto)).
+            assert (H1 : map (@proj1_sig _ _) (f split) = map (@proj1_sig _ _) split)
+              by (clear; abstract (induction split; simpl; f_equal; auto)).
+            rewrite <- H0; clear H0.
+            rewrite <- H1; clear H1.
+            generalize (f split); clear split; clear f.
+            intros fsplit pats.
+            clear pf.
+            revert pats str.
+            induction fsplit;
+              intro pats; intros;
+              destruct pats;
+              repeat match goal with
+                       | [ H : @eq nat _ _ |- _ ] => progress simpl in H
+                       | [ H : @eq nat _ _ |- _ ] => exfalso; revert H; clear; intro H; abstract inversion H
+                       | _ => progress subst
+                       | [ H : S _ = S _ |- _ ] => apply (f_equal pred) in H
+                       | [ H : ?x = ?x |- _ ] => clear H
+                     end.
+            { simpl in *; left; subst... }
+            { simpl in *.
+              let IHfsplit := match goal with
+                                | [ IHfsplit : forall pats str,
+                                                 ilist _ _ ->
+                                                 _ = _ ->
+                                                 fold_right _ _ _ = str ->
+                                                 _ + _
+                                                 |- _ ] => constr:IHfsplit
+                              end in
+              match goal with
+                | [ H : Datatypes.length _ = Datatypes.length _ |- _ ]
+                  => specialize (fun l => IHfsplit _ _ l H eq_refl)
+              end;
+                let ls := match goal with | [ ls : ilist _ (_::_) |- _ ] => constr:ls end in
+                specialize (IHfsplit (ilist_tl ls));
+                  let ls_hd := fresh "ls_hd" in
+                  pose proof (ilist_hd ls) as ls_hd;
+                    simpl in ls_hd;
+                    clear ls;
+                    refine (match ls_hd, IHfsplit with
+                              | inl p1, inl p2 => inl (ParseApp p1 p2)
+                              | inr _, _ => inr None
+                              | _, inr _ => inr None
+                            end). } } }
+      { (** decide_leaf *)
+        intros str ch.
+        case_eq (str =s [[ch]]); intro H; [ apply bool_eq_correct in H; left | right; exact None ].
+        subst... }
+      { (** fold_patterns *)
+        intros str pats parses; induction parses; simpl in *;
+        repeat match goal with
+                 | [ H : option _ |- _ ] => destruct H
+                 | [ H : sum _ _ |- _ ] => destruct H
+               end;
+          try solve [ left; auto with parse_tree nocore
+                    | left;
+                      repeat match goal with
+                               | _ => progress auto with parse_tree nocore
+                               | [ H : parse_of _ _ _ _ |- _ ] => inversion H; clear H; subst
+                             end
+                    | match goal with
+                        | [ H : parse_of _ _ _ _ |- _ ] => fail 1
+                        | _ => idtac
+                      end;
+                      right; exact None
+                    | right;
+                      apply Some;
+                      let p := fresh in
+                      intro p; inversion p; clear p; subst;
+                      auto with parse_tree nocore ]. }
+      { (** make_abort *)
+        intros; exact None. }
+    Defined.
+  End parse_tree.
+
+
+(*  Section parse_tree_no_split.
+    Local Hint Constructors parse_of parse_of_pattern parse_of_item : parse_tree.
+    Local Hint Resolve ParseHead ParsePatternSingleton : parse_tree.
+    Local Hint Extern 1 => apply ParseHead : parse_tree.
+    Local Hint Extern 0 (option (parse_of _ _ _ [])) => exact None : parse_tree.
+
+    Definition parse_tree_no_split_for : forall str nt, option (parse_of String G str nt).
+    Proof with auto with parse_tree nocore.
+      apply (@parse_nonterminal (fun str nt => option (parse_of _ G str nt))).
+      { intros str name [p|]; [ apply Some | exact None ]... }
+      { intros.
+        specialize (parse_pattern_from_split_list' ((exist _ str pf)::nil) pat); simpl in *.
+        destruct pat as [|pat0 [|pat1 pats] ]; simpl in *.
+        { case_eq (str =s Empty _); intro H; [ apply Some | exact None ]...
+          apply bool_eq_correct in H; subst... }
+        { destruct (ilist_hd parse_pattern_from_split_list') as [tree|]; simpl in *; [ apply Some | exact None ]... }
+        { (** we don't handle the case where we need to split the string *)
+          exact None. } }
+      { (** decide_leaf *)
+        intros str ch.
+        case_eq (str =s [[ch]]); intro H; [ apply bool_eq_correct in H; apply Some | exact None ].
+        subst... }
+      { (** fold_patterns *)
+        intros str pats parses; induction parses; simpl in *...
+        repeat match goal with H : option _ |- _ => destruct H end;
+          try solve [ apply Some; auto with parse_tree nocore
+                    | apply Some;
+                      repeat match goal with
+                               | _ => progress auto with parse_tree nocore
+                               | [ H : parse_of _ _ _ _ |- _ ] => inversion H; clear H; subst
+                             end
+                    | match goal with
+                        | [ H : parse_of _ _ _ _ |- _ ] => fail 1
+                        | _ => idtac
+                      end;
+                      exact None ]. }
+      { (** make_abort *)
+        intros; exact None. }
+    Defined.
+  End parse_tree_no_split.
+
+
+
+
+  Section generic_by_simple_listing.
+    (** If we don't need to pass proofs down the tree, we can just ask for a list of splits. *)
+    Context (T_success T_failure : String -> nonterminal CharType -> Type)
+            (T_success_reverse_lookup : forall str name, T_success str (Lookup G name) -> T_success str [ [ NonTerminal _ name ] ])
+            (T_failure_reverse_lookup : forall str name, T_failure str (Lookup G name) -> T_failure str [ [ NonTerminal _ name ] ])
+            (transport_T_success_str : forall (s1 s2 : String) nt, s1 = s2 -> T_success s1 nt -> T_success s2 nt)
+            (transport_T_failure_str : forall (s1 s2 : String) nt, s1 = s2 -> T_failure s1 nt -> T_failure s2 nt).
+    Let T str nt := (T_success str nt + T_failure str nt)%type.
+    Let transport_T_str (s1 s2 : String) nt (H : s1 = s2) (p : T s1 nt) : T s2 nt :=
+      match p with
+        | inl p' => inl (transport_T_success_str H p')
+        | inr p' => inr (transport_T_failure_str H p')
+      end.
+    Context (pick_patterns
+             : forall (str : String)
+                      (pat : pattern CharType),
+                 { ls : list { split : list { str_part : String | Length _ str_part < Length _ str \/ str_part = str }
+                             | List.length split = List.length pat
+                               /\ fold_right (Concat _) (Empty _) (map (@proj1_sig _ _) split) = str }
+                 | List.length ls <> 0 }).
+    Context (simple_fold_pattern_parts
+             : forall str0
+                      strs
+                      (pat : pattern CharType)
+                      (pf : List.length strs = List.length pat),
+                 ilist (fun sp : {str1 : String |
+                                  Length String str1 < Length String str0 \/
+                                  str1 = str0} * item CharType
+                        => T (proj1_sig (fst sp)) [ [ snd sp ] ])
+                       (combine strs pat)
+                 -> T (fold_left (Concat _) (map (@proj1_sig _ _) strs) (Empty _))
+                      [ pat ]).
+    Context (decide_leaf : forall str ch, T str [ [ Terminal ch ] ]).
+    Context (fold_patterns : forall str (pats : list (pattern CharType)),
+                               ilist (fun pat => T str [ pat ]) pats
+                               -> T str pats).
+    Context (make_abort : forall str nt valid_list, @is_valid_nonterminal str valid_list nt = false -> T_failure str nt).
+
+    Definition parse_nonterminal_with_split_picker str nt : T str nt.
+    Proof.
+      refine (@parse_nonterminal T_success T_failure T_success_reverse_lookup T_failure_reverse_lookup transport_T_success_str transport_T_failure_str _ decide_leaf fold_patterns make_abort str nt).
+      clear str nt.
+      intros str0 parse_a_split str H pat.
+      specialize (pick_patterns str pat).
+      specialize (fun strs => parse_a_split strs pat).
+      specialize (fun strs H =>
+                    @simple_fold_pattern_parts _ _ _ H (parse_a_split strs)).
+      clear parse_a_split.
+      move simple_fold_pattern_parts at bottom.
+      specialize (fun strs pf1 pf2 =>
+                    @transport_T_str
+                      _ str _ pf1
+                      (@simple_fold_pattern_parts strs pf2)).
+      clear simple_fold_pattern_parts.
+      move pick_patterns at bottom.
+      move transport_T_str at bottom.
+      destruct pick_patterns as [ls H'].
+      let T := match type of ls with list (@sig (list ?T) _) => constr:(T) end in
+      set (f := (map (fun x' : T
+                      => exist
+                           (fun str => Length String str < Length String str0 \/ str = str0)
+                           (proj1_sig x')
+                           (match H, proj2_sig x' with
+                              | or_introl H0, or_introl H1 => or_introl (transitivity H1 H0)
+                              | or_introl H0, or_intror H1 => or_introl (transitivity (R := le) (Le.le_n_S _ _ (NPeano.Nat.eq_le_incl _ _ (f_equal (Length String) H1))) H0)
+                              | or_intror H0, or_introl H1 => or_introl (transitivity (R := le) H1 (NPeano.Nat.eq_le_incl _ _ (f_equal (Length String) H0)))
+                              | or_intror H0, or_intror H1 => or_intror (transitivity H1 H0)
+                            end)))).
+      pose proof (map f (map (@proj1_sig _ _) ls)).
+      let T := match type of ls with list ?T => constr:(T) end in
+      pose proof (@map
+                    T _
+                    f
+                    ls).
+
+      assert (forall B : Type, ({split
+       : list
+           {str_part : String |
+           Length String str_part < Length String str \/ str_part = str} |
+       Datatypes.length split = Datatypes.length pat /\
+       fold_left (Concat String)
+         (map
+            (proj1_sig
+               (P:=fun str_part : String =>
+                   Length String str_part < Length String str \/
+                   str_part = str)) split) (Empty String) = str} -> B)).
+      intros B x.
+      assert (list
+    {str_part : String |
+     Length String str_part < Length String str \/ str_part = str} ->
+              list {str : String | Length String str < Length String str0 \/ str = str0}).
+      refine .
+      SearchAbout (_ <= _ -> S _ <= S _).
+
+      refine (fun x' => _).
+      refine (map _
+                   pose proof (@transport_T_str (map (fun x' => exist _ (proj1_sig x') (proj1_sig x)).
+ in parse
+
+
+
+      apply simple_fold_pattern_parts.
+
+      move pick_patterns at bottom.
+      pose @imap_list.
+            := @parse_nonterminal_or_abort str str initial_nonterminal_data
+                                           (or_intror eq_refl) nt.
 
   Section parse_tree_no_split.
     Local Hint Constructors parse_of parse_of_pattern parse_of_item : parse_tree.
@@ -298,6 +606,48 @@ Section recursive_descent_parser.
         intros; exact None. }
     Defined.
   End parse_tree_no_split.
+
+
+  Section parse_tree_no_split.
+    Local Hint Constructors parse_of parse_of_pattern parse_of_item : parse_tree.
+    Local Hint Resolve ParseHead ParsePatternSingleton : parse_tree.
+    Local Hint Extern 1 => apply ParseHead : parse_tree.
+    Local Hint Extern 0 (option (parse_of _ _ _ [])) => exact None : parse_tree.
+
+    Definition parse_tree_no_split_for : forall str nt, option (parse_of String G str nt).
+    Proof with auto with parse_tree nocore.
+      apply (@parse_nonterminal (fun str nt => option (parse_of _ G str nt))).
+      { intros str name [p|]; [ apply Some | exact None ]... }
+      { intros.
+        specialize (parse_pattern_from_split_list' ((exist _ str pf)::nil) pat); simpl in *.
+        destruct pat as [|pat0 [|pat1 pats] ]; simpl in *.
+        { case_eq (str =s Empty _); intro H; [ apply Some | exact None ]...
+          apply bool_eq_correct in H; subst... }
+        { destruct (ilist_hd parse_pattern_from_split_list') as [tree|]; simpl in *; [ apply Some | exact None ]... }
+        { (** we don't handle the case where we need to split the string *)
+          exact None. } }
+      { (** decide_leaf *)
+        intros str ch.
+        case_eq (str =s [[ch]]); intro H; [ apply bool_eq_correct in H; apply Some | exact None ].
+        subst... }
+      { (** fold_patterns *)
+        intros str pats parses; induction parses; simpl in *...
+        repeat match goal with H : option _ |- _ => destruct H end;
+          try solve [ apply Some; auto with parse_tree nocore
+                    | apply Some;
+                      repeat match goal with
+                               | _ => progress auto with parse_tree nocore
+                               | [ H : parse_of _ _ _ _ |- _ ] => inversion H; clear H; subst
+                             end
+                    | match goal with
+                        | [ H : parse_of _ _ _ _ |- _ ] => fail 1
+                        | _ => idtac
+                      end;
+                      exact None ]. }
+      { (** make_abort *)
+        intros; exact None. }
+    Defined.
+  End parse_tree_no_split.*)
 End recursive_descent_parser.
 
 Section recursive_descent_parser_list.
@@ -443,10 +793,142 @@ Section
 *)
 
 
-Module example_parse_empty_grammar.
-  Definition make_parse_of : forall str nt, option (parse_of string_stringlike (trivial_grammar _) str nt).
+Section example_parse_string_grammar.
+  Fixpoint make_all_single_splits (str : string) : list { strs : string * string | (fst strs ++ snd strs = str)%string }.
   Proof.
-    eapply parse_tree_no_split_for
+    refine ((exist _ (""%string, str) eq_refl)::_).
+    refine (match str with
+              | ""%string => nil
+              | String.String ch str' => map (fun p => exist _ (String.String ch (fst (proj1_sig p)),
+                                                                snd (proj1_sig p))
+                                                             _)
+                                             (make_all_single_splits str')
+            end).
+    simpl; apply f_equal.
+    apply proj2_sig.
+  Defined.
+
+  Lemma length_append (s1 s2 : string) : length (s1 ++ s2) = length s1 + length s2.
+  Proof.
+    revert s2.
+    induction s1; simpl; trivial; [].
+    intros.
+    f_equal; auto.
+  Qed.
+
+  Fixpoint flatten1 {T} (ls : list (list T)) : list T
+    := match ls with
+         | nil => nil
+         | x::xs => (x ++ flatten1 xs)%list
+       end.
+
+  Lemma flatten1_length_ne_0 {T} (ls : list (list T)) (H0 : Datatypes.length ls <> 0)
+        (H1 : Datatypes.length (hd nil ls) <> 0)
+  : Datatypes.length (flatten1 ls) <> 0.
+  Proof.
+    destruct ls as [| [|] ]; simpl in *; auto.
+  Qed.
+
+  Local Ltac t' :=
+    match goal with
+      | _ => progress simpl in *
+      | _ => progress subst
+      | [ H : ?a = ?b |- _ ] => progress subst a
+      | [ H : ?a = ?b |- _ ] => progress subst b
+      | _ => rewrite (LeftId string_stringlike _)
+      | _ => rewrite (RightId string_stringlike _)
+      | _ => reflexivity
+      | _ => split
+      | _ => right; reflexivity
+      | _ => rewrite map_length
+      | _ => rewrite map_map
+      | _ => rewrite length_append
+      | _ => progress destruct_head_hnf prod
+      | _ => progress destruct_head_hnf and
+      | _ => progress destruct_head_hnf or
+      | _ => progress destruct_head_hnf sig
+      | _ => progress auto with arith
+      | _ => apply f_equal
+      | _ => solve [ apply proj2_sig ]
+      | _ => solve [ left; auto with arith ]
+      | [ str : string |- _ ] => solve [ destruct str; simpl; auto with arith ]
+      | [ str : string |- _ ] => solve [ left; destruct str; simpl; auto with arith ]
+    end.
+  Local Ltac t'' :=
+    match goal with
+      | _ => progress t'
+      | [ str : string |- _ ] => solve [ destruct str; repeat t' ]
+    end.
+  Local Ltac t :=
+    solve [ repeat t'' ].
+
+  Local Hint Resolve NPeano.Nat.lt_lt_add_l NPeano.Nat.lt_lt_add_r NPeano.Nat.lt_add_pos_r NPeano.Nat.lt_add_pos_l : arith.
+
+  Definition brute_force_splitter
+  : forall (str : string_stringlike) (pat : pattern Ascii.ascii),
+      Datatypes.length pat > 0 ->
+      {ls
+       : list
+           {split
+            : list
+                {str_part : string_stringlike |
+                 Length string_stringlike str_part < Length string_stringlike str \/
+                 str_part = str} |
+            Datatypes.length split = Datatypes.length pat /\
+            fold_right (Concat string_stringlike) (Empty string_stringlike)
+                       (map (@proj1_sig _ _) split) = str} |
+       Datatypes.length ls <> 0}.
+  Proof.
+    simpl.
+    intros str [|pat pats] H;
+      [ exfalso; clear str; simpl in H; abstract inversion H
+      | clear H ].
+    revert str.
+    induction pats; simpl in *; intros str.
+    { (** We only get one thing in the list *)
+      refine (exist _ ((exist _ ((exist _ str _)::nil) _)::nil) _).
+      simpl; auto with arith. }
+    { pose (make_all_single_splits str) as single_splits.
+      pose proof (map (@proj1_sig _ _) single_splits).
+      pose proof (fun str => map (map (@proj1_sig _ _)) (map (@proj1_sig _ _) (proj1_sig (IHpats str)))).
+      let P := match goal with |- sig ?P => constr:P end in
+      refine (exist
+                P
+                (flatten1
+                   (map (fun s1s2p =>
+                           map
+                             (fun split_list => exist
+                                                  _
+                                                  (((exist _ (fst (proj1_sig s1s2p)) _)
+                                                      ::(map (fun s => exist _ (proj1_sig s) _)
+                                                             (proj1_sig split_list))))
+                                                  _)
+                             (proj1_sig (IHpats (snd (proj1_sig s1s2p)))))
+                        single_splits))
+                _).
+      apply flatten1_length_ne_0; simpl.
+      { rewrite !map_length; subst_body; simpl; clear;
+        abstract (destruct str; simpl; auto with arith). }
+      { subst_body;
+        destruct str; simpl.
+        { rewrite map_length; clear; abstract t. }
+        { rewrite map_length; clear; abstract t. } } }
+    Grab Existential Variables.
+    { simpl. split.
+      { rewrite map_length; clear; abstract t. }
+      { subst_body; rewrite map_map; simpl; abstract t. } }
+    { abstract t. }
+    { abstract t. }
+    { simpl; abstract t. }
+    { abstract t. }
+  Defined.
+
+  Variable G : grammar Ascii.ascii.
+
+  Definition brute_force_make_parse_of : forall str nt, parse_of string_stringlike G str nt
+                                            + option (parse_of string_stringlike G str nt -> False).
+  Proof.
+    eapply parse_tree_for
     with (nonterminal_listT := rdp_list_nonterminal_listT)
            (is_valid_nonterminal := rdp_list_is_valid_nonterminal Ascii.ascii_dec)
            (remove_nonterminal := rdp_list_remove_nonterminal Ascii.ascii_dec)
@@ -454,6 +936,84 @@ Module example_parse_empty_grammar.
     { intros; exact [Lookup (trivial_grammar _) ""%string]. }
     { apply rdp_list_remove_nonterminal_dec. }
     { apply rdp_list_ntl_wf. }
+    { apply brute_force_splitter. }
+  Defined.
+End example_parse_string_grammar.
+
+Module example_parse_empty_grammar.
+  Definition make_parse_of : forall str nt, parse_of string_stringlike (trivial_grammar _) str nt
+                                            + option (parse_of string_stringlike (trivial_grammar _) str nt -> False)
+    := brute_force_make_parse_of _.
+
+
+
+  Definition parse : forall str : string,
+                       (parse_of string_stringlike (trivial_grammar _) str (trivial_grammar _))
+                       + option ((parse_of string_stringlike (trivial_grammar _) str (trivial_grammar _)) -> False)
+    := fun str => make_parse_of str _.
+
+  Eval hnf in if (parse "") then true else false.
+  Eval hnf in if (parse "a") then true else false.
+
+  Arguments eq_rect_r / .
+  Arguments eq_rec_r / .
+  Arguments eq_ind_r / .
+
+  Goal True.
+    pose (parse "") as X.
+    hnf in X; simpl in X.
+    pose (parse "a") as Y.
+    hnf in Y; simpl in Y.
+  Abort.
+End example_parse_empty_grammar.
+
+(*
+
+Module example_parse_empty_grammar.
+  Definition make_parse_of : forall str nt, parse_of string_stringlike (trivial_grammar _) str nt
+                                            + option (parse_of string_stringlike (trivial_grammar _) str nt -> False).
+  Proof.
+    eapply parse_tree_for
+    with (nonterminal_listT := rdp_list_nonterminal_listT)
+           (is_valid_nonterminal := rdp_list_is_valid_nonterminal Ascii.ascii_dec)
+           (remove_nonterminal := rdp_list_remove_nonterminal Ascii.ascii_dec)
+           (nonterminal_listT_R := rdp_list_nonterminal_listT_R).
+    { intros; exact [Lookup (trivial_grammar _) ""%string]. }
+    { apply rdp_list_remove_nonterminal_dec. }
+    { apply rdp_list_ntl_wf. }
+    { simpl.
+      intros str pat H.
+      refine (exist _ (_::nil) _).
+      exact (NPeano.Nat.neq_succ_0 _).
+      Grab Existential Variables.
+      hnf in pat.
+      destruct pat as [|pat pats];
+        simpl in *;
+        [ exfalso; revert H; clear; intro H; abstract inversion H
+        | clear H ].
+      revert str.
+      induction pats.
+      { simpl; intros str.
+        refine (exist _ ((exist _ str _)::nil) (conj eq_refl (RightId string_stringlike _))). }
+      { simpl in *; intros str.
+        destruct str as [|ch str].
+        { specialize (IHpats ""%string).
+          destruct IHpats as [split [H0 H1] ].
+          exists ((exist _ ""%string (or_intror eq_refl))::split); simpl;
+          split; f_equal; auto. }
+        { specialize (IHpats str); simpl.
+          destruct IHpats as [split [H0 H1] ].
+          destruct str; simpl in *.
+          { exists ((exist _ (String.String ch ""%string) (or_intror eq_refl))::split);
+            split; simpl; try solve [ f_equal; auto ]. }
+        simpl in *.
+        simpl.
+        exact .
+
+
+      SearchAbout (_ ++ "")%string.
+      simpl.
+      SearchAbout (S _ <> 0).
   Defined.
 
   Definition parse : forall str : string,
@@ -470,3 +1030,4 @@ Module example_parse_empty_grammar.
     hnf in Y; simpl in Y.
   Abort.
 End example_parse_empty_grammar.
+*)
